SSProve/Hax/TPhase/DropReferences.lean
@@ -36,6 +36,8 @@ def tDropReferences : TExpr → TExpr
   | .mk (.assign n rhs) ty => .mk (.assign n (tDropReferences rhs)) ty
   | .mk (.forLoop v lo hi body) ty =>
       .mk (.forLoop v (tDropReferences lo) (tDropReferences hi) (tDropReferences body)) ty
+  | .mk (.forLoopRev v lo hi body) ty =>
+      .mk (.forLoopRev v (tDropReferences lo) (tDropReferences hi) (tDropReferences body)) ty
   | .mk (.whileLoop c body) ty =>
       .mk (.whileLoop (tDropReferences c) (tDropReferences body)) ty
   | .mk (.break_ (some e)) ty => .mk (.break_ (some (tDropReferences e))) ty
@@ -45,10 +47,14 @@ def tDropReferences : TExpr → TExpr
   | .mk (.questionMark e) ty => .mk (.questionMark (tDropReferences e)) ty
   | .mk (.forFold v lo hi body) ty =>
       .mk (.forFold v (tDropReferences lo) (tDropReferences hi) (tDropReferences body)) ty
+  | .mk (.forFoldRev v lo hi body) ty =>
+      .mk (.forFoldRev v (tDropReferences lo) (tDropReferences hi) (tDropReferences body)) ty
   | .mk (.whileFold c body) ty =>
       .mk (.whileFold (tDropReferences c) (tDropReferences body)) ty
   | .mk (.forFoldReturn v lo hi body) ty =>
       .mk (.forFoldReturn v (tDropReferences lo) (tDropReferences hi) (tDropReferences body)) ty
+  | .mk (.forFoldRevReturn v lo hi body) ty =>
+      .mk (.forFoldRevReturn v (tDropReferences lo) (tDropReferences hi) (tDropReferences body)) ty
   | .mk (.whileFoldReturn c body) ty =>
       .mk (.whileFoldReturn (tDropReferences c) (tDropReferences body)) ty
   | .mk (.cfBreak e) ty => .mk (.cfBreak (tDropReferences e)) ty
@@ -91,6 +97,8 @@ theorem tDropReferences_erase (e : TExpr) :
   | assign _ _ _ ih => simp [tDropReferences, TExpr.erase, dropReferences, ih]
   | forLoop _ _ _ _ _ ih1 ih2 ih3 =>
     simp [tDropReferences, TExpr.erase, dropReferences, ih1, ih2, ih3]
+  | forLoopRev _ _ _ _ _ ih1 ih2 ih3 =>
+    simp [tDropReferences, TExpr.erase, dropReferences, ih1, ih2, ih3]
   | whileLoop _ _ _ ih1 ih2 =>
     simp [tDropReferences, TExpr.erase, dropReferences, ih1, ih2]
   | break_some _ _ ih => simp [tDropReferences, TExpr.erase, dropReferences, ih]
@@ -98,9 +106,13 @@ theorem tDropReferences_erase (e : TExpr) :
   | questionMark _ _ ih => simp [tDropReferences, TExpr.erase, dropReferences, ih]
   | forFold _ _ _ _ _ ih1 ih2 ih3 =>
     simp [tDropReferences, TExpr.erase, dropReferences, ih1, ih2, ih3]
+  | forFoldRev _ _ _ _ _ ih1 ih2 ih3 =>
+    simp [tDropReferences, TExpr.erase, dropReferences, ih1, ih2, ih3]
   | whileFold _ _ _ ih1 ih2 =>
     simp [tDropReferences, TExpr.erase, dropReferences, ih1, ih2]
   | forFoldReturn _ _ _ _ _ ih1 ih2 ih3 =>
+    simp [tDropReferences, TExpr.erase, dropReferences, ih1, ih2, ih3]
+  | forFoldRevReturn _ _ _ _ _ ih1 ih2 ih3 =>
     simp [tDropReferences, TExpr.erase, dropReferences, ih1, ih2, ih3]
   | whileFoldReturn _ _ _ ih1 ih2 =>
     simp [tDropReferences, TExpr.erase, dropReferences, ih1, ih2]
